src/test/bigram.test.lean
@@ -1,0 +1,21 @@
+import ..bigram ..equate
+
+open robot tactic
+constant α : Type
+constants A B C : set α
+run_cmd (do 
+    rt ← robot.get_equate_rule_table,
+    bgc ← bigram.of_rule_table rt,
+    tactic.trace $ bigram.bigram_cache.occs bgc,
+    tactic.trace $ bigram.bigram_cache.trigs bgc,
+    b1 ← tactic.to_expr ```(A ∩ (B ∪ C)),
+    b2 ← tactic.to_expr ```(A ∪ (B ∩ C)),
+    -- -- b2 ← bigram.of_names `has_inter.inter `has_union.union,
+    -- -- let b1 : bigram := bigram.mk `(has_union.union) `(has_union.union),
+    d1 ← bigram.distance bgc b1 b2,
+    tactic.trace d1, 
+    pure ()
+)
+
+
+
